disk-betree/BlockCacheSystemCrashSafeBlockInterfaceRefinement.dfy
@@ -1,17 +1,145 @@
 include "BlockCacheSystem.dfy"
 include "CrashSafe.dfy"
+include "../lib/Maps.dfy"
 
 module BlockCacheSystemCrashSafeBlockInterfaceRefinement {
   import BCS = BlockCacheSystem
   import CSBI = CrashSafeBlockInterface
 
+  import opened Maps
+
+  import BC = BlockCache
+  import BI = BlockInterface
+  import D = Disk
+  import DiskBetree
+  type Node<Value> = DiskBetree.Node<Value>
+  type Reference = BI.Reference
+  type DiskOp<T> = BC.DiskOp<T>
+
   function Ik(k: BCS.Constants) : CSBI.Constants
   {
-    CSBI.Constants(k.machine.constants, k.machine.constants)
+    k.machine.constants
   }
 
-  function I(k: BCS.Constants, s: BCS.Variables) : CSBI.Variables
+  function RefGraph(m: map<Reference, Node>) : imap<Reference, iset<Reference>>
   {
+    imap ref | ref in m :: BC.Successors(m[ref])
+  }
+
+  function I<Value>(k: BCS.Constants, s: BCS.Variables) : CSBI.Variables<Node<Value>>
+  requires BCS.Inv(k, s)
+  {
+    var persistentGraph := BCS.PersistentGraph(k, s);
+    var ephemeralGraph := if s.machine.Ready? then BCS.EphemeralGraph(k, s) else persistentGraph;
     CSBI.Variables(
+      BI.Variables(
+        MapToImap(persistentGraph),
+        RefGraph(persistentGraph)
+      ),
+      BI.Variables(
+        MapToImap(ephemeralGraph),
+        RefGraph(ephemeralGraph)
+      )
+    )
+  }
+
+  lemma RefinesInit(k: BCS.Constants, s: BCS.Variables)
+  requires BCS.Init(k, s)
+  ensures BCS.Inv(k, s)
+  ensures CSBI.Init(Ik(k), I(k, s))
+
+  lemma RefinesWriteBack(k: BCS.Constants, s: BCS.Variables, s': BCS.Variables, dop: DiskOp, ref: Reference)
+  requires BCS.Inv(k, s)
+  requires BCS.Inv(k, s')
+  requires BC.WriteBack(k.machine, s.machine, s'.machine, dop, ref)
+  requires D.Write(k.disk, s.disk, s'.disk, dop)
+  ensures CSBI.Next(Ik(k), I(k, s), I(k, s'))
+  {
+    assert I(k, s).persistent == I(k, s').persistent;
+    //assert BI.NextStep(I(k, s).ephemeral, I(k, s').ephemeral, BI.Stutter);
+    //assert CSBI.NextStep(Ik(k), I(k, s), I(k, s'), CSBI.EphemeralMoveStep);
+  }
+
+  lemma RefinesWriteBackSuperblock(k: BCS.Constants, s: BCS.Variables, s': BCS.Variables, dop: DiskOp)
+  requires BCS.Inv(k, s)
+  requires BCS.Inv(k, s')
+  requires BC.WriteBackSuperblock(k.machine, s.machine, s'.machine, dop)
+  requires D.Write(k.disk, s.disk, s'.disk, dop)
+  ensures CSBI.Next(Ik(k), I(k, s), I(k, s'))
+
+  lemma RefinesDirty(k: BCS.Constants, s: BCS.Variables, s': BCS.Variables, dop: DiskOp, ref: Reference, block: Node)
+  requires BCS.Inv(k, s)
+  requires BCS.Inv(k, s')
+  requires BC.Dirty(k.machine, s.machine, s'.machine, dop, ref, block)
+  requires D.Stutter(k.disk, s.disk, s'.disk, dop)
+  ensures CSBI.Next(Ik(k), I(k, s), I(k, s'))
+
+  lemma RefinesAlloc(k: BCS.Constants, s: BCS.Variables, s': BCS.Variables, dop: DiskOp, ref: Reference, block: Node)
+  requires BCS.Inv(k, s)
+  requires BCS.Inv(k, s')
+  requires BC.Alloc(k.machine, s.machine, s'.machine, dop, ref, block)
+  requires D.Stutter(k.disk, s.disk, s'.disk, dop)
+  ensures CSBI.Next(Ik(k), I(k, s), I(k, s'))
+
+  lemma RefinesUnalloc(k: BCS.Constants, s: BCS.Variables, s': BCS.Variables, dop: DiskOp, ref: Reference)
+  requires BCS.Inv(k, s)
+  requires BCS.Inv(k, s')
+  requires BC.Unalloc(k.machine, s.machine, s'.machine, dop, ref)
+  requires D.Stutter(k.disk, s.disk, s'.disk, dop)
+  ensures CSBI.Next(Ik(k), I(k, s), I(k, s'))
+
+  lemma RefinesPageIn(k: BCS.Constants, s: BCS.Variables, s': BCS.Variables, dop: DiskOp, ref: Reference)
+  requires BCS.Inv(k, s)
+  requires BCS.Inv(k, s')
+  requires BC.PageIn(k.machine, s.machine, s'.machine, dop, ref)
+  requires D.Read(k.disk, s.disk, s'.disk, dop)
+  ensures CSBI.Next(Ik(k), I(k, s), I(k, s'))
+
+  lemma RefinesPageInSuperblock(k: BCS.Constants, s: BCS.Variables, s': BCS.Variables, dop: DiskOp)
+  requires BCS.Inv(k, s)
+  requires BCS.Inv(k, s')
+  requires BC.PageInSuperblock(k.machine, s.machine, s'.machine, dop)
+  requires D.Read(k.disk, s.disk, s'.disk, dop)
+  ensures CSBI.Next(Ik(k), I(k, s), I(k, s'))
+
+  lemma RefinesEvict(k: BCS.Constants, s: BCS.Variables, s': BCS.Variables, dop: DiskOp, ref: Reference)
+  requires BCS.Inv(k, s)
+  requires BCS.Inv(k, s')
+  requires BC.Evict(k.machine, s.machine, s'.machine, dop, ref)
+  requires D.Stutter(k.disk, s.disk, s'.disk, dop)
+  ensures CSBI.Next(Ik(k), I(k, s), I(k, s'))
+
+  lemma RefinesCrashStep(k: BCS.Constants, s: BCS.Variables, s': BCS.Variables)
+  requires BCS.Inv(k, s)
+  requires BCS.Inv(k, s')
+  requires BC.Init(k.machine, s'.machine)
+  requires s.disk == s'.disk
+  ensures CSBI.Next(Ik(k), I(k, s), I(k, s'))
+
+  lemma RefinesNextStep(k: BCS.Constants, s: BCS.Variables, s': BCS.Variables, step: BCS.Step)
+  requires BCS.Inv(k, s)
+  requires BCS.NextStep(k, s, s', step)
+  ensures BCS.Inv(k, s')
+  ensures CSBI.Next(Ik(k), I(k, s), I(k, s'))
+  {
+    BCS.NextPreservesInv(k, s, s');
+    match step {
+      case MachineStep(dop: DiskOp) => {
+        var mstep :| BC.NextStep(k.machine, s.machine, s'.machine, dop, mstep);
+        match mstep {
+          case WriteBackStep(ref) => RefinesWriteBack(k, s, s', dop, ref);
+          case WriteBackSuperblockStep => RefinesWriteBackSuperblock(k, s, s', dop);
+          case DirtyStep(ref, block) => RefinesDirty(k, s, s', dop, ref, block);
+          case AllocStep(ref, block) => RefinesAlloc(k, s, s', dop, ref, block);
+          case UnallocStep(ref) => RefinesUnalloc(k, s, s', dop, ref);
+          case PageInStep(ref) => RefinesPageIn(k, s, s', dop, ref);
+          case PageInSuperblockStep => RefinesPageInSuperblock(k, s, s', dop);
+          case EvictStep(ref) => RefinesEvict(k, s, s', dop, ref);
+        }
+      }
+      case CrashStep => {
+        RefinesCrashStep(k, s, s');
+      }
+    }
   }
 }
